src/Impl_vm.v
@@ -29,15 +29,35 @@ Fixpoint copland_compile (t:AnnoTerm): CVM unit :=
       e <- get_ev ;;
       p <- get_pl ;;
       pr <- split_ev x sp e p ;;
-      let '(e1,e2) := pr in
-      put_ev e1 ;;
+      let '(e2,et2) := pr in
+      (*put_ev e1 ;; *)
       copland_compile t1 ;;
       e1r <- get_ev ;;
+      e1rt <- get_evT ;;
       put_ev e2 ;;
+      put_evT et2 ;;
       copland_compile t2 ;;
       e2r <- get_ev ;;
-      join_seq (Nat.pred y) p e1r e2r
+      e2rt <- get_evT ;;
+      join_seq (Nat.pred y) p e1r e1rt e2r e2rt
   | abpar (x,y) sp t1 t2 =>
+    e <- get_ev ;;
+    p <- get_pl ;;
+    pr <- split_ev x sp e p ;;
+    let '(e2,et2) := pr in
+    (*put_ev e1 ;; *)
+    copland_compile t1 ;;
+    e1r <- get_ev ;;
+    e1rt <- get_evT ;;
+    put_ev e2 ;;
+    put_evT et2 ;;
+    copland_compile t2 ;;
+    e2r <- get_ev ;;
+    e2rt <- get_evT ;;
+    join_par (Nat.pred y) p e1r e1rt e2r e2rt
+
+
+    (*
       e <- get_ev ;;
       p <- get_pl ;;
       pr <- split_ev x sp e p ;;
@@ -48,7 +68,7 @@ Fixpoint copland_compile (t:AnnoTerm): CVM unit :=
       put_ev e2 ;;
       copland_compile t2 ;;
       e2r <- get_ev ;;
-      join_par (Nat.pred y) p e1r e2r
+      join_par (Nat.pred y) p e1r e2r *)
   end.
 
 Definition run_cvm (t:AnnoTerm) st : cvm_st :=
