src/StVM.v
@@ -12,9 +12,10 @@ Import ListNotations.
 (* Specific VM monad state *)
 (*Definition ev_store := MapC nat EvidenceC. *)
 Record cvm_st : Type := mk_st
-                         {st_ev:EvidenceC ;
-                          st_trace:list Ev ;
-                          st_pl:Plc (*;
-                          st_store:ev_store*)}.
+                          {st_ev:EvidenceC ;
+                           st_evT: Evidence ;
+                           st_trace:list Ev ;
+                           st_pl:Plc (*;
+                           st_store:ev_store*)}.
 
-Definition empty_vmst := mk_st mtc [] 0 (* [] *) .
+Definition empty_vmst := mk_st mtc mt [] 0 (* [] *) .
